lakefile.lean
@@ -6,10 +6,10 @@ package «reflection» {
 }
 
 -- require std from git "https://github.com/leanprover/std4" @ "nightly-testing-2024-04-04"
-require aesop from git "https://github.com/JLimperg/aesop" @ "v4.12.0"
+-- require aesop from git "https://github.com/JLimperg/aesop" @ "v4.12.0"
 -- require IIT from git "https://github.com/arthur-adjedj/iit" @ "v4.4.0"
 -- require Qq from git "https://github.com/leanprover-community/quote4" @ "53156671405fbbd5402ed17a79bd129b961bd8d6"
--- require mathlib from git "https://github.com/leanprover-community/mathlib4" @ "v4.8.0"
+require mathlib from git "https://github.com/leanprover-community/mathlib4" @ "bump/v4.12.0"
 -- require auto from git "https://github.com/leanprover-community/lean-auto" @ "v4.11.0" -- doesn't work from lean 4.8
 
 @[default_target]
